Defined [StepM], an ordinary state transition step

src/Reduction.v
@@ -1,76 +1,74 @@
 Require Import Bool List String Peano_dec.
-Require Import Common ListSupport FMap Syntax Semantics StepT SemFacts.
+Require Import Common ListSupport FMap Syntax Semantics StepM SemFacts.
 
 Set Implicit Arguments.
 
-Ltac dest_step_t :=
+Ltac dest_step_m :=
   repeat match goal with
-         | [H: steps step_t _ _ _ _ |- _] => inv H
-         | [H: step_t _ _ _ _ |- _] => inv H
-         | [H: {| tst_oss := _ |} = {| tst_oss := _ |} |- _] => inv H
+         | [H: steps step_m _ _ _ _ |- _] => inv H
+         | [H: step_m _ _ _ _ |- _] => inv H
+         | [H: {| bst_oss := _ |} = {| bst_oss := _ |} |- _] => inv H
          end; simpl in *.
 
-Definition EquivTState (tst1 tst2: TState) :=
-  tst_oss tst1 = tst_oss tst2 /\
-  tst_orqs tst1 = tst_orqs tst2 /\
-  EquivMP (tst_msgs tst1) (tst_msgs tst2) /\
-  tst_tid tst1 = tst_tid tst2.
+Definition EquivMState (st1 st2: MState) :=
+  bst_oss st1 = bst_oss st2 /\
+  bst_orqs st1 = bst_orqs st2 /\
+  EquivMP (bst_msgs st1) (bst_msgs st2).
 
 Ltac dest_equivT :=
   repeat
     match goal with
-    | [H: EquivTState _ _ |- _] => red in H; dest; simpl in *; subst
+    | [H: EquivMState _ _ |- _] => red in H; dest; simpl in *; subst
     | [H: ?t = ?t |- _] => clear H
     end.
 
 Ltac split_equivT :=
-  split; [|split; [|split]]; simpl.
+  split; [|split]; simpl.
 
-Lemma EquivTState_refl:
-  forall tst, EquivTState tst tst.
+Lemma EquivMState_refl:
+  forall st, EquivMState st st.
 Proof.
   intros; split_equivT; auto.
   apply EquivMP_refl.
 Qed.
 
-Lemma EquivTState_sym:
-  forall tst1 tst2, EquivTState tst1 tst2 -> EquivTState tst2 tst1.
+Lemma EquivMState_sym:
+  forall st1 st2, EquivMState st1 st2 -> EquivMState st2 st1.
 Proof.
   intros; dest_equivT; split_equivT; auto.
   apply EquivMP_sym; auto.
 Qed.
 
-Lemma EquivTState_trans:
-  forall tst1 tst2 tst3,
-    EquivTState tst1 tst2 ->
-    EquivTState tst2 tst3 ->
-    EquivTState tst1 tst3.
+Lemma EquivMState_trans:
+  forall st1 st2 st3,
+    EquivMState st1 st2 ->
+    EquivMState st2 st3 ->
+    EquivMState st1 st3.
 Proof.
   intros; dest_equivT; split_equivT.
   - rewrite H; auto.
-  - rewrite H4; auto.
+  - rewrite H3; auto.
   - eapply EquivMP_trans; eauto.
-  - rewrite H6; auto.
 Qed.
 
-Lemma EquivTState_step_t:
+Lemma EquivMState_step_m:
   forall sys st1 lbl st2,
-    step_t sys st1 lbl st2 ->
+    step_m sys st1 lbl st2 ->
     forall cst1,
-      EquivTState st1 cst1 ->
+      EquivMState st1 cst1 ->
       exists cst2,
-        step_t sys cst1 lbl cst2 /\ EquivTState st2 cst2.
+        step_m sys cst1 lbl cst2 /\ EquivMState st2 cst2.
 Proof.
   intros.
   inv H.
   - exists cst1; split; auto.
     constructor.
-  - destruct cst1 as [coss1 corqs1 cmsgs1 cts1].
+  - destruct cst1 as [coss1 corqs1 cmsgs1].
     dest_equivT; eexists; split.
     + econstructor; eauto.
     + split_equivT; auto.
       apply EquivMP_enqMP; auto.
-  - destruct cst1 as [coss1 corqs1 cmsgs1 cts1].
+  - destruct cst1 as [coss1 corqs1 cmsgs1].
     dest_equivT; eexists; split.
     + econstructor; try reflexivity; try eassumption.
       eapply EquivMP_Forall_FirstMP; eauto.
@@ -80,54 +78,54 @@ Proof.
       auto.
 Qed.
 
-Lemma EquivTState_steps_t:
+Lemma EquivMState_steps_t:
   forall sys st1 hst st2,
-    steps step_t sys st1 hst st2 ->
+    steps step_m sys st1 hst st2 ->
     forall cst1,
-      EquivTState st1 cst1 ->
+      EquivMState st1 cst1 ->
       exists cst2,
-        steps step_t sys cst1 hst cst2 /\ EquivTState st2 cst2.
+        steps step_m sys cst1 hst cst2 /\ EquivMState st2 cst2.
 Proof.
   induction 1; simpl; intros.
   - exists cst1; split; auto.
     constructor.
   - specialize (IHsteps _ H1); destruct IHsteps as [csti [? ?]].
-    eapply EquivTState_step_t in H0; eauto.
+    eapply EquivMState_step_m in H0; eauto.
     destruct H0 as [cst2 [? ?]].
     eexists; split.
     + econstructor; eassumption.
     + assumption.
 Qed.
 
-Definition msgAddrOf {MsgT} `{HasMsg MsgT} (msg: MsgT) :=
-  mid_addr (msg_id (getMsg msg)).
+Definition msgAddrOf (msg: Msg) :=
+  mid_addr (msg_id msg).
 
-Definition NonSilentHistory (hst: THistory) :=
-  Forall (fun tlbl => tlbl <> emptyRLabel) hst.
+Definition NonSilentHistory (hst: History) :=
+  Forall (fun lbl => lbl <> emptyRLabel) hst.
 
-Definition NotMsgIn {MsgT} (lbl: RLabel MsgT) :=
+Definition NotMsgIn (lbl: MLabel) :=
   match lbl with
   | RlblIn _ => False
   | _ => True
   end.
 
-Definition NonMsgInHistory (hst: THistory) :=
+Definition NonMsgInHistory (hst: History) :=
   Forall (fun tlbl => NotMsgIn tlbl) hst.
 
 Lemma msg_in_commutes:
-  forall sys st1 emsg tlbl st2,
-    NotMsgIn tlbl ->
-    steps step_t sys st1 [RlblIn emsg; tlbl] st2 ->
+  forall sys st1 emsg lbl st2,
+    NotMsgIn lbl ->
+    steps step_m sys st1 [RlblIn emsg; lbl] st2 ->
     forall cst1,
-      EquivTState st1 cst1 ->
+      EquivMState st1 cst1 ->
       exists cst2,
-        steps step_t sys cst1 [tlbl; RlblIn emsg] cst2 /\
-        EquivTState st2 cst2.
+        steps step_m sys cst1 [lbl; RlblIn emsg] cst2 /\
+        EquivMState st2 cst2.
 Proof.
   intros.
-  destruct tlbl as [|hdl mins mouts]; [elim H|].
-  destruct cst1 as [coss1 corqs1 cmsgs1 cts1].
-  dest_step_t.
+  destruct lbl as [|hdl mins mouts]; [elim H|].
+  destruct cst1 as [coss1 corqs1 cmsgs1].
+  dest_step_m.
   - eexists; split.
     + repeat econstructor; eauto.
     + dest_equivT.
@@ -152,40 +150,28 @@ Proof.
         do 2 rewrite <-app_assoc.
         apply EquivMP_app.
         { apply EquivMP_removeMsgs; auto. }
-        { assert (NoDup
-                    (map msgAddrOf
-                         (intOuts
-                            sys (toTMsgs match getTMsgsTInfo mins with
-                                         | Some ti => ti
-                                         | None => {| tinfo_tid := nts;
-                                                      tinfo_rqin := map tmsg_msg mins |}
-                                         end outs)))).
+        { assert (NoDup (map msgAddrOf (intOuts sys mouts))).
           { apply NoDup_map_filter.
-            apply MsgAddr_NoDup_toTMsg.
-            eapply ValidMsgOuts_MsgAddr_NoDup; eauto.
+            eapply ValidMsgOuts_MsgAddr_NoDup in H17; eauto.
           }
-          assert (NoDup ((map msgAddrOf [toTMsgU emsg0]))) by (repeat constructor; auto).
+          assert (NoDup ((map msgAddrOf [emsg])))
+            by (repeat constructor; auto).
           assert (DisjList
-                    (map msgAddrOf
-                         (intOuts
-                            sys (toTMsgs match getTMsgsTInfo mins with
-                                         | Some ti => ti
-                                         | None => {| tinfo_tid := nts;
-                                                      tinfo_rqin := map tmsg_msg mins |}
-                                         end outs)))
-                    (map msgAddrOf [toTMsgU emsg0])).
-          { assert (mid_from (msg_id (getMsg emsg0)) <> rule_oidx rule).
+                    (map msgAddrOf (intOuts sys mouts))
+                    (map msgAddrOf [emsg])).
+          { assert (mid_from (msg_id emsg) <> rule_oidx rule).
             { unfold fromExternal, isExternal in H2.
+              simpl in H2; unfold id in H2.
               intro Hx; rewrite Hx in H2.
-              destruct (rule_oidx rule ?<n indicesOf sys); [discriminate|auto].
+              destruct (rule_oidx rule ?<n sys_inds sys); [discriminate|auto].
             }
-            destruct H16.
+            destruct H17.
 
             clear -H7 H8.
-            induction outs; [apply DisjList_nil_1|].
-            inv H8; specialize (IHouts H2); dest.
+            induction mouts; [apply DisjList_nil_1|].
+            inv H8; specialize (IHmouts H2); dest.
             unfold DisjList in *; intros.
-            specialize (IHouts e); destruct IHouts; auto.
+            specialize (IHmouts e); destruct IHmouts; auto.
             destruct (ma_from e ==n rule_oidx rule).
             { right; intro Hx; Common.dest_in; auto. }
             { left; intro Hx; simpl in Hx.
@@ -207,55 +193,55 @@ Qed.
 
 Lemma msg_in_reduced:
   forall sys st1 emsg hst2 st2,
-    steps step_t sys st1 (RlblIn emsg :: hst2) st2 ->
+    steps step_m sys st1 (RlblIn emsg :: hst2) st2 ->
     NonMsgInHistory hst2 ->
     forall cst1,
-      EquivTState st1 cst1 ->
+      EquivMState st1 cst1 ->
       exists cst2,
-        steps step_t sys cst1 (hst2 ++ [RlblIn emsg]) cst2 /\
-        EquivTState st2 cst2.
+        steps step_m sys cst1 (hst2 ++ [RlblIn emsg]) cst2 /\
+        EquivMState st2 cst2.
 Proof.
-  induction hst2 as [|tlbl ?]; simpl; intros.
-  - dest_step_t.
-    destruct cst1 as [coss1 corqs1 cmsgs1 cts1].
-    exists {| tst_oss := coss1; tst_orqs := corqs1;
-              tst_msgs := enqMP (toTMsgU emsg0) cmsgs1; tst_tid := cts1 |}; split.
+  induction hst2 as [|lbl ?]; simpl; intros.
+  - dest_step_m.
+    destruct cst1 as [coss1 corqs1 cmsgs1].
+    exists {| bst_oss := coss1; bst_orqs := corqs1;
+              bst_msgs := enqMP emsg cmsgs1 |}; split.
     + repeat econstructor; eauto.
     + dest_equivT; split_equivT; auto.
       apply EquivMP_enqMP; auto.
       
   - inv H0.
-    change (RlblIn emsg :: tlbl :: hst2) with ([RlblIn emsg; tlbl] ++ hst2) in H.
+    change (RlblIn emsg :: lbl :: hst2) with ([RlblIn emsg; lbl] ++ hst2) in H.
     eapply steps_split in H; [|reflexivity].
     destruct H as [sti [? ?]].
-    eapply msg_in_commutes in H0; [|assumption|apply EquivTState_refl].
+    eapply msg_in_commutes in H0; [|assumption|apply EquivMState_refl].
     destruct H0 as [cst2 [? ?]].
     pose proof (steps_append H H0); inv H3.
     specialize (IHhst2 _ H9 H5 _ H1).
     destruct IHhst2 as [icst2 [? ?]].
-    eapply EquivTState_step_t in H11; [|eassumption].
+    eapply EquivMState_step_m in H11; [|eassumption].
     destruct H11 as [cst3 [? ?]].
     exists cst3; split.
     + econstructor; eauto.
-    + eapply EquivTState_trans; eauto.
+    + eapply EquivMState_trans; eauto.
 Qed.
 
 Lemma msg_in_reduced_app:
   forall sys st1 hst1 emsg hst2 st2,
-    steps step_t sys st1 (hst1 ++ RlblIn emsg :: hst2) st2 ->
+    steps step_m sys st1 (hst1 ++ RlblIn emsg :: hst2) st2 ->
     NonMsgInHistory hst2 ->
     forall cst1,
-      EquivTState st1 cst1 ->
+      EquivMState st1 cst1 ->
       exists cst2,
-        steps step_t sys cst1 (hst1 ++ hst2 ++ [RlblIn emsg]) cst2 /\
-        EquivTState st2 cst2.
+        steps step_m sys cst1 (hst1 ++ hst2 ++ [RlblIn emsg]) cst2 /\
+        EquivMState st2 cst2.
 Proof.
   intros.
   eapply steps_split in H; [|reflexivity].
   destruct H as [sti [? ?]].
   eapply msg_in_reduced in H; eauto.
   destruct H as [csti [? ?]].
-  eapply EquivTState_steps_t in H2; eauto.
+  eapply EquivMState_steps_t in H2; eauto.
   destruct H2 as [cst2 [? ?]].
   exists cst2; split.
   - eapply steps_append; eauto.
@@ -264,20 +250,20 @@ Qed.
 
 Lemma msg_outs_commutes:
   forall sys st1 rule1 mins1 mouts1 rule2 mins2 mouts2 st2,
-    steps step_t sys st1 [RlblOuts (Some rule1) mins1 mouts1;
+    steps step_m sys st1 [RlblOuts (Some rule1) mins1 mouts1;
                             RlblOuts (Some rule2) mins2 mouts2] st2 ->
     rule_oidx rule1 <> rule_oidx rule2 ->
     DisjList (map msgAddrOf mouts2) (map msgAddrOf mins1) ->
     forall cst1,
-      EquivTState st1 cst1 ->
+      EquivMState st1 cst1 ->
       exists cst2,
-        steps step_t sys cst1 [RlblOuts (Some rule2) mins2 mouts2;
+        steps step_m sys cst1 [RlblOuts (Some rule2) mins2 mouts2;
                                  RlblOuts (Some rule1) mins1 mouts1] cst2 /\
-        EquivTState st2 cst2.
+        EquivMState st2 cst2.
 Proof.
   (* intros. *)
   (* destruct cst1 as [coss1 corqs1 cmsgs1 cts1]. *)
-  (* dest_step_t. *)
+  (* dest_step_m. *)
   (* eexists; split. *)
   (* - dest_equivT. *)
   (*   econstructor. *)
