src/StepM.v
@@ -1,0 +1,37 @@
+Require Import Bool List String Peano_dec.
+Require Import Common FMap Syntax Semantics.
+
+Inductive step_m (sys: System): MState -> MLabel -> MState -> Prop :=
+| SmSlt: forall st, step_m sys st emptyRLabel st
+| SmExt: forall pst nst oss orqs oims emsg,
+    fromExternal sys emsg = true ->
+    toInternal sys emsg = true ->
+    pst = {| bst_oss := oss; bst_orqs := orqs; bst_msgs := oims |} ->
+    nst = {| bst_oss := oss;
+             bst_orqs := orqs;
+             bst_msgs := enqMP emsg oims
+          |} ->
+    step_m sys pst (RlblIn emsg) nst
+| SmInt: forall pst nst oss orqs oims oidx os porq pos norq msgs rule outs,
+    oidx = rule_oidx rule ->
+    In oidx (indicesOf sys) ->
+    oss@[oidx] = Some os ->
+    orqs@[oidx] = Some porq ->
+    Forall (FirstMP oims) msgs ->
+    ValidMsgsIn oidx msgs ->
+    map (fun tmsg => msg_id tmsg) msgs = rule_mids rule ->
+    In rule (sys_rules sys) ->
+    rule_precond rule os porq msgs ->
+    rule_postcond rule os porq msgs pos norq outs ->
+    ValidMsgOuts oidx outs ->
+
+    pst = {| bst_oss := oss; bst_orqs := orqs; bst_msgs := oims |} ->
+    nst = {| bst_oss := oss +[ oidx <- pos ];
+             bst_orqs := orqs +[ oidx <- norq ];
+             bst_msgs := distributeMsgs
+                           (intOuts sys outs)
+                           (removeMsgs msgs oims)
+          |} ->
+
+    step_m sys pst (RlblOuts (Some rule) msgs outs) nst.
+
